James C - swapped order of type checking and pattern matching

isabelle/Chapter12_2_PatternMatching.thy
@@ -1,5 +1,5 @@
-theory Chapter12_3_PatternMatching
-imports Chapter12_2_Typechecking
+theory Chapter12_2_PatternMatching
+imports Chapter12_1_Language
 begin
 
 type_synonym substitution = "expr list"
@@ -7,14 +7,6 @@ type_synonym substitution = "expr list"
 primrec apply_subst :: "substitution => expr => expr"
 where "apply_subst [] e = e"
     | "apply_subst (s # sig) e = apply_subst sig (subst (mult_insert (length sig) s) e)"
-
-inductive typecheck_subst :: "type env => substitution => type env => bool"
-where tc_sub_nil [simp]: "typecheck_subst gam [] empty_env"
-    | tc_sub_cons [simp]: "typecheck gam e t ==> typecheck_subst gam es sig ==> 
-          typecheck_subst gam (e # es) (extend sig t)"
-
-inductive_cases [elim!]: "typecheck_subst g [] sig"
-inductive_cases [elim!]: "typecheck_subst g (e # es) sig"
 
 inductive matches :: "patn => expr => substitution => bool"
 where [simp]: "matches VarPat e [e]"
@@ -39,20 +31,5 @@ where "no_match p1 e1 ==> no_match (PairPat p1 p2) (Pair e1 e2)"
     | "no_match p e ==> no_match (InLPat p) (InL t t' e)"
     | "no_match (InRPat p) (InL t t' e)"
     | "no_match p e ==> no_match (InRPat p) (InR t t' e)"
-
-lemma [simp]: "typecheck_subst gam s sig ==> length s = env_size sig"
-by (induction gam s sig rule: typecheck_subst.induct, simp_all)
-
-lemma [simp]: "typecheck_subst gg s g ==> typecheck_subst gg s' g' ==> 
-        typecheck_subst gg (s @ s') (g +++ g')"
-by (induction s g rule: typecheck_subst.induct, simp_all) 
-
-lemma [simp]: "typecheck_subst gam s sig ==> typecheck (sig +++ gam) e t ==> 
-        typecheck gam (apply_subst s e) t"
-by (induction gam s sig arbitrary: e rule: typecheck_subst.induct, simp_all)
-
-lemma [simp]: "matches p e s ==> typecheck gam e t1 ==> typecheck_patn p t1 sig ==> 
-        typecheck_subst gam s sig"
-by (induction p e s arbitrary: gam t1 sig rule: matches.induct, auto)
 
 end
